eIris/tests/inductive_list_2.v
@@ -1,0 +1,72 @@
+From elpi Require Import elpi.
+From iris.proofmode Require Import proofmode tactics coq_tactics reduction.
+From iris.prelude Require Import options.
+From iris.bi Require Import fixpoint.
+From iris.algebra Require Import ofe monoid list.
+From iris.heap_lang Require Import proofmode.
+From iris.heap_lang Require Import notation.
+From stdpp Require Import base finite.
+
+Context `{!heapGS Σ}.
+Notation iProp := (iProp Σ).
+Implicit Types l : loc.
+
+
+Definition is_list_pre_lgfp (is_list : val → iProp) : val → iProp := (λ hd,
+  ⌜hd = NONEV⌝
+  ∨ 
+  ∃ l tl v, ⌜hd = SOMEV #l⌝ ∗ l ↦ (v,tl) ∗ is_list tl)%I.
+
+Local Lemma is_list_pre_lgfp_mono (is_list1 is_list2 : val -d> iProp): 
+  ⊢ (□ ∀ hd, is_list1 hd -∗ is_list2 hd) → 
+    ∀ hd, is_list_pre_lgfp is_list1 hd -∗ is_list_pre_lgfp is_list2 hd.
+Proof.
+  iIntros "#H"; iIntros (hd) "HF1".
+  rewrite /is_list_pre_lgfp.
+  iDestruct "HF1" as "[HF1|HF1]".
+  - eauto.
+  - iDestruct "HF1" as "[%l [%tl [%v (Hhd & HP & HL2)]]]".
+    iRight.
+    iExists l, tl, v.
+    iFrame.
+    by iApply "H".
+Qed.
+
+(* Definition is_list_pre_lgfp' : 
+  (val -d> iProp) →
+  val -d> iProp :=
+    uncurry ∘ is_list_pre_lgfp ∘ curry.
+
+Local Instance is_list_pre_lgfp_mono' : BiMonoPred is_list_pre_lgfp'.
+Proof.
+  constructor.
+  - iIntros (is_list1 is_list2 ??) "#H".
+    iIntros ([hd vs]); iRevert (hd vs).
+    iApply is_list_pre_lgfp_mono.
+    iIntros "!>" (hd vs).
+    iApply "H".
+  - intros is_list Hne n [hd vs] [hd' vs'] [Hhd Hvs]; simplify_eq /=.
+    rewrite /curry /is_list_pre_lgfp.
+    revert Hvs; revert vs'.
+    induction vs as [|v vs IH]; intros vs' Hvs; setoid_rewrite list_dist_Forall2 in Hvs. 
+    + apply Forall2_nil_inv_l in Hvs. 
+      simplify_eq. 
+      setoid_rewrite Hhd.
+      f_equiv.
+    + inversion Hvs; simplify_eq /=.
+      setoid_rewrite H1.
+      setoid_rewrite Hhd.
+      repeat f_equiv.
+      by apply list_dist_Forall2.
+Qed. *)
+
+Definition is_list_lfp_def := λ hd, bi_least_fixpoint is_list_pre_lgfp' (hd, vs).
+Definition is_list_gfp_def := λ hd, bi_greatest_fixpoint is_list_pre_lgfp' (hd, vs).
+
+Lemma is_list_lfp_unfold hd vs :
+  is_list_lfp_def hd vs ⊣⊢ is_list_pre_lgfp is_list_lfp_def hd vs.
+Proof. by rewrite /is_list_lfp_def least_fixpoint_unfold. Qed.
+
+Lemma is_list_gfp_unfold hd vs :
+  is_list_gfp_def hd vs ⊣⊢ is_list_pre_lgfp is_list_gfp_def hd vs.
+Proof. by rewrite /is_list_gfp_def greatest_fixpoint_unfold. Qed.
